\documentclass{_mypackages/monograph}

\title{Useful equations} % \MyTitle
\author{Bruno Murino} % \MyAuthor
\date{\today} % \MyDate

% \addbibresource{qinfo.bib}

\begin{document}

\chapter*{Useful equations}

\section*{Math}

\begin{equation}
    \int_{-\infty}^\infty \dd{p} \exp{ipx} = 2\pi \delta(x)
\end{equation}

\begin{equation}
    \int_{-\infty}^{\infty} \dd{x} \exp{-ax^2 + bx} = \sqrt{\frac{\pi}{a}} \lexp\left(\frac{b^2}{4a}\right) \qc \Re(a)>0
\end{equation}

\begin{equation}
    \comm{AB}{CD} = A\comm{B}{C}D + \comm{A}{C}BD + CA\comm{B}{D} + C\comm{A}{D}B
\end{equation}

\begin{equation}
    \exp{t(X+Y)} = \exp{tX}\exp{tY}\exp{-\frac{t^2}{2}\comm{X}{Y}}\exp{\,
\frac{t^3}{3!}(2\comm{Y}{\comm{X}{Y}}+\comm{X}{\comm{X}{Y}})}\cdots
\end{equation}

\begin{equation}
    \int_{-\infty}^{\infty} \dd{x} x\exp{-ax^2 + bx} =\frac{b}{2} \sqrt{\frac{\pi}{a^3}} \lexp\left(\frac{b^2}{4a}\right) \qc \Re(a)>0
\end{equation}

\begin{equation}
    \int_{-\infty}^{\infty} \dd{x} x^2\exp{-ax^2 + bx} =\frac{2a+b^2}{4} \sqrt{\frac{\pi}{a^5}} \lexp\left(\frac{b^2}{4a}\right) \qc \Re(a)>0
\end{equation}

\begin{equation}
    \frac{1}{1-x} = \sum_{n=0}^\infty x^n
\end{equation}

\begin{equation}
\begin{split}
    \sum_{n=0}^\infty \left(\frac{\rho}{2}\right)^n \frac{1}{n!} \lexp\left(-\frac{(x^2 + x'^2)}{2}\right) &H_n(x) H_n(x') =\\ 
    &\frac{\rho^{-1/2}}{\sqrt{\rho^{-1}-\rho}} \lexp\left(  \frac{4xx' - (\rho^{-1}+\rho)(x^2 + x'^2)}{2(\rho^{-1}-\rho)} \right).
\end{split}
\end{equation}

\begin{equation}
    \int_{-\infty}^\infty \dd{x} H_m(x) H_n(x) \exp{-x^2} = \sqrt{\pi} 2^n n! \delta_{nm}
\end{equation}

\begin{equation}
    \sinh(x) = \sum_{n=0}^\infty \frac{x^{2n+1}}{(2n+1)!}\qc \cosh(x) = \sum_{n=0}^\infty \frac{x^{2n}}{(2n)!}
\end{equation}

\begin{equation}
    \sin(x) = \sum_{n=0}^\infty \frac{i^{2n}\, x^{2n+1}}{(2n+1)!}\qc \cos(x) = \sum_{n=0}^\infty \frac{i^{2n}\, x^{2n}}{(2n)!}
\end{equation}

\begin{equation}
    \exp{B}A\exp{-B} = A + \comm{B}{A} + \frac{1}{2!} \comm{B}{\comm{B}{A}} + \frac{1}{3!}\comm{B}{\comm{B}{\comm{B}{A}}} + \cdots
\end{equation}

\begin{equation}
    (\vb{a}\cross \vb{b})_k = \epsilon_{ijk}\,a_i\,b_j
\end{equation}

If \(\comm{A}{B}=C\) and \(\comm{A}{C} = \comm{B}{C}=0\):
\begin{equation}
    \exp{A+B}=\exp{A}\exp{B}\exp{-\hlf C}
\end{equation}

If \(\comm{A}{B}=C\) and \(\comm{A}{\comm{A}{C}} = \comm{A}{\comm{B}{C}} = \comm{B}{\comm{B}{C}}=0\):
\begin{equation}
    \exp{A+B} = \exp{A}\exp{B}\exp{-\hlf C}\exp{\frac{1}{3}\comm{B}{C}}\exp{\frac{1}{6}\comm{A}{C}}
\end{equation}

\begin{equation}
    (y-a)f(y)=0 \Rightarrow f(y) = \delta(y-a)
\end{equation}































































\section*{Physics}

\begin{equation}
    U(t,t_0) = \exp{-i(t-t_0)H}
\end{equation}

\begin{equation}
    J(x,t;x',t') = \mel{x}{U(t,t')}{x'}
\end{equation}

\begin{equation}
    \psi(x,t) = \int \dd{x'} \bigg(\mel{x}{U(t,t')}{x'} \bigg)\psi(x',t')
\end{equation}

\begin{equation}
    \sigma_0 = \mqty(\pmat{0}) \qc \sigma_x = \mqty(\pmat{1}) \qc \sigma_y = \mqty(\pmat{2}) \qc \sigma_z = \mqty(\pmat{3}) 
\end{equation}

\begin{equation}
    \sigma_{+} = \frac{\sigma_x + i \sigma_y}{2} = \ketbra{0}{1} = \mqty(0 & 1 \\ 0 & 0) \qc \sigma_{-} = \frac{\sigma_x - i \sigma_y}{2} = \ketbra{1}{0} = \mqty(0 & 0 \\ 1 & 0),
\end{equation}

\begin{equation}
    \comm{\sigma_i}{\sigma_j} = 2\, i\, \epsilon_{ijk}\sigma_k \qc \comm{\sigma_{+}}{\sigma_{-}} = \sigma_z \qc
    \comm{\sigma_{z}}{\sigma_{\pm}} = \pm 2\, \sigma_{\pm}
\end{equation}

\begin{equation}
    \sigma_x^2 = \sigma_y^2 = \sigma_z^2 = -i\sigma_x \sigma_y \sigma_z = \idm \qc \det(\sigma_i) = -1\qc \Tr(\sigma_i) = 0
\end{equation}

\begin{equation}
    \vb{n}\cdot\bm{\sigma} = \mqty(n_z & n_x - in_y \\ n_x + in_y & -n_z)\qc \det(\vb{n}\cdot\bm{\sigma}) = -\abs{\vb{n}}^2
\end{equation}

\begin{equation}
    (\vb{n}\cdot\bm{\sigma})^{2n} = \idm \qc \exp{i\theta\,  (\vb{n}\cdot\bm{\sigma})} = \cos(\theta) + i (\vb{n}\cdot\bm{\sigma}) \sin(\theta)\qc \abs{\vb{n}} = 1
\end{equation}

\begin{equation}
    \braket{\vb{x}}{\vb{p}} = \frac{1}{(2\pi)^{\nicefrac{3}{2}}}\lexp{(i\, \va{p}\cdot\va{x}})\qc \va{p},\va{x} \in \R^3
\end{equation}

\begin{equation}
    \vb{p}\ket{\vb{x}} = i \pdv{\vb{x}} \ket{\vb{x}} \qc \bra{\vb{x}}\vb{p} = -i \pdv{\vb{x}} \bra{\vb{x}}.
\end{equation}

\begin{equation}
    \vb{x}\ket{\vb{p}} = -i \pdv{\vb{p}} \ket{\vb{p}} \qc \bra{\vb{p}}\vb{x} = i \pdv{\vb{p}} \bra{\vb{p}}.
\end{equation}

\begin{equation}
    \comm{Q}{P} = i\hbar 
\end{equation}

\begin{equation}
    \comm{F(\vb{x})}{p_i} = i\hbar \pdv{F(\vb{x})}{x_i}\qc \comm{x_i}{F(\vb{p})} = i\hbar \pdv{F(\vb{p})}{p_i}
\end{equation}

\begin{equation}
    q = \sqrt{\frac{m\omega}{\hbar}} Q = \frac{1}{\sqrt{2}}(a^\dagger + a) \qc p = \frac{P}{\sqrt{m\omega \hbar }} = \frac{i}{\sqrt{2}}(a^\dagger - a) \qc \comm{q}{p} = i
\end{equation}

\begin{equation}
    a = \frac{1}{\sqrt{2}}(q + i p) \qc a^\dagger = \frac{1}{\sqrt{2}}(q - i p) \qc \comm{a}{a^\dagger} = 1
\end{equation}

\begin{equation}
    N \ket{n} = a^\dagger a \ket{n} = n \ket{n}\qc a \ket{n} = \sqrt{n}\ket{n-1}\qc a^\dagger \ket{n} = \sqrt{n+1}\ket{n+1}
\end{equation}

\begin{equation}
    H = \frac{\omega}{2}(p^2 + q^2) = \omega(N+\hlf)
\end{equation}

\begin{equation}
    \comm{N}{a} = -a\qc \comm{N}{a^\dagger} = a^\dagger\qc a\ket{0} = 0 \qc \ket{n} = \frac{(a^\dagger)^n}{\sqrt{n!}}\ket{0}
\end{equation}

\begin{equation}
    \braket{x}{n} = \frac{\pi^{-1/4}}{\sqrt{2^n n!}} \lexp\left(-\frac{x^2}{2}\right)H_n(x)
\end{equation}

\begin{equation}
    \exp{-i\gamma px}x\exp{i\gamma px} = \exp{-i\gamma xp}x\exp{i\gamma xp}  = \exp{-\gamma}x
\end{equation}

\begin{equation}
    \exp{-i\gamma px}\ket{p} = \exp{-\gamma}\ket{\exp{-\gamma}p}
\end{equation}

\begin{equation}
    \exp{-i\gamma px}p\exp{i\gamma px} = \exp{-i\gamma xp}p\exp{i\gamma xp}  = \exp{\gamma}p
\end{equation}

\begin{equation}
    \exp{-i\theta(\vb{T}\cdot \vu{n})} = \Big[\idm - (\vb{T}\cdot \vu{n})^2 \Big] + \Big[\cos \theta (\vb{T}\cdot \vu{n})^2 - i\sin \theta (\vb{T}\cdot \vu{n})\Big]
\end{equation}

\begin{equation}
    \exp{-i\theta(\vb{T}\cdot \vu{n})} = \idm - i\sin \theta (\vb{T}\cdot \vu{n}) - (1-\cos \theta)(\vb{T}\cdot\vu{n})^2
\end{equation}

\section*{Angular Momentum}

\begin{equation}
    J_\pm \ket{jm} = \sqrt{j(j+1)-m(m\pm1)}\ket{jm\pm1} = \sqrt{(j\mp m)(j\pm m + 1)}\ket{jm\pm1}
\end{equation}


% \backmatter
% \printbib
\end{document}
